src/ObcToClight/Generation.v
@@ -465,7 +465,8 @@ Definition translate (do_sync: bool) (all_public: bool)
         let f_gvar := (f, type_of_inst main_node) in
         let ins := map glob_bind m.(m_in) in
         let outs := map glob_bind m.(m_out) in
-        (* let prog := rev prog in *)
+        (* revert the declarations ! *)
+        let prog := rev prog in
         let cs := map (translate_class prog) prog in
         let (structs, funs) := split cs in
         let main := (main_id, make_main false main_node m) in
